<?xml version="1.0" encoding="UTF-8"?>

<section xml:id="sec-10-2" xmlns:xi="http://www.w3.org/2001/XInclude">
    <title>PMI</title>

    <p>I'm just going to write what I put in my notes and let you pick what you want from it, because it seems a little incomplete.</p>

<section xml:id="sec-10-5">
    <title>Introducing PMI</title>
    
    <p>Principle of Mathematic Induction. How it works: Let <m>S</m> be a subset of <m>\mathbb{N}</m> with these properties:</p>
    <ol>
        <li>
            <p><m>1 \in S</m>; and</p>
        </li>
        <li>
            <p>for all <m>n \in \mathbb{N}</m>, if <m>n \in S</m>, then <m>n+1 \in S</m></p>
        </li>
    </ol>
    <p>Then <m>S=\mathbb{N}</m></p>

    <p>Here's how a proof of <m>(\forall n \in \mathbb{N}) P(n)</m> by mathematical induction works.</p>
    <ol marker="i.)">
        <li>
            <p>Show that <m>P(1)</m> is true. This is the <term>basis step</term>.</p>
        </li>
        <li>
            <p>Suppose <m>P(n)</m> is true. This is the <term>induction assumption</term>.</p>
            <me>\vdots</me>
        </li>
        <li>
            <p>Conclude <m>P(n+1)</m> is true.</p>
        </li>
        <li>
            <p>Therefore, by the principle of mathematical induction, <m>(\forall n \in \mathbb{N}) P(n)</m> is true.</p>
        </li>
    </ol>

</section>

<section>
    <title>2 PMI proofs</title>
        <p><alert>Prove:</alert> <m>\forall n \in \mathbb{N} </m> (for every natural number) 
            <m>\sum_{i=1}^{n} 2i-1 = n^2</m></p>
        <proof>
            <p><alert>Basis step:</alert> show it's true for 1</p>
            <p>Let <m>n=1</m>. Calculate <m>\sum_{i=1}^{1} 2i-1 = (1)^2</m> :</p>
            <me>2(1)-1=1</me>
            <p><alert>Inductive step:</alert> assume it's true for <m>n</m></p>
            <p>Let <m>n \in \mathbb{N}</m> where <m>n&gt; 1</m> and assume <m>\sum_{i=1}^{n} 2i-1 = n^2</m>. Calculate:</p>
            <me>(n+1)^2 = n^2 +2n +1</me>
            <p>Now we <em>show</em> it's true for <m>n+1</m>:</p>
            <p>Calculate:</p>
            <md>
                <mrow>\sum_{i=1}^{n+1} 2i-1 = (n+1)^2 \amp= [\sum_{i=1}^{n} 2i-1]+(2(n+1)-1)</mrow>
                <mrow>\amp=n^2 \text{ (from induction assumption) } + (2(n+1)-1)</mrow>
                <mrow>\amp=n^2+2n+2-1</mrow>
                <mrow>\amp=n^2+2n+1</mrow>
                <mrow>\amp=(n+1)^2</mrow>
            </md>
            <p>Thus, by principle of mathematical induction, <m>\sum_{i=1}^{n+1} 2i-1 = (n+1)^2</m>. Hence, by proof by 
                principle of mathematical induction, <m>\sum_{i=1}^{n} 2i-1 = n^2</m> for all natural numbers. <m>\square</m></p>
            
        </proof>

        <proof>
            <p><alert>Prove:</alert> <m>\forall n\in \mathbb{N}</m>  <m>\prod_{i=1}^{n} (4i-2) = \frac{2n!}{n!}</m></p>
            <p><alert>Basis step:</alert> show it's true for 1</p>
            <p>Let <m>n=1</m>. Calculate <m>\prod_{i=1}^{1} (4i-2) = \frac{2(1)!}{(1)!}</m> :</p>
            <me>4(1)-2=2</me>
            <p><alert>Inductive step:</alert> assume it's true for <m>n</m></p>
            <p>Let <m>n \in \mathbb{N}</m> where <m>n&gt; 1</m> and assume <m>\prod_{i=1}^{n} (4i-2) = \frac{2n!}{n!}</m>. Calculate:</p>
            <me>\prod_{i=1}^{n+1} (4i-2) = \frac{2(n+1)!}{(n+1)!}</me>
            <p>Now we <em>show</em> it's true for <m>n+1</m>:</p>
            <p>Calculate:</p>
            <md>
                <mrow>\prod_{i=1}^{n+1} (4i-2) = \frac{2(n+1)!}{(n+1)!} \amp= (\prod_{i=1}^{n} (4i-2))((4(n+1)-2)</mrow>
                <mrow>\amp=\frac{2n!}{n!} \text{ (from induction assumption) }((4(n+1)-2)</mrow>
                <mrow>\amp=(\frac{2n!}{n!})(4n+2)</mrow>
                <mrow>\amp=(\frac{2n!}{n!})(2(2n+1))</mrow>
                <mrow>\amp=(2)\frac{(2n+1)((2n)!)}{n!}</mrow>
                <mrow>\amp=\frac{(2n+1)!}{n!}(2)</mrow>
                <mrow>\amp=\frac{(2n+2)!}{\frac{1}{2}(2n+2)n!}</mrow>
                <mrow>\amp=\frac{(2n+2)!}{(n+1)n!}</mrow>
                <mrow>\amp=\frac{(2n+2)!}{(n+1)!}</mrow>
            </md>
            <p>Thus, by principle of mathematical induction, <m>\prod_{i=1}^{n+1} (4i-2) = \frac{2(n+1)!}{(n+1)!}</m>.</p>
            <p>Hence, by proof by principle of mathematical induction, <m>\prod_{i=1}^{n} (4i-2) = \frac{2n!}{n!}</m>. <m>\square</m></p>


        </proof>


</section>

<section>
    <p>
        <alert>Generalized principle of Mathematical Induction</alert>
    </p>
    <p>Let <m>k</m> be a natural number. Let <m>S</m> be a subset of <m>\mathbb{N}</m> with these two properties:</p>
    <ol marker="i.)">
        <li><m>k\in S</m>; and</li>
        <li><m>\forall n \in \mathbb{N}</m> with <m>n \geq k</m>, if <m>n \in S</m>, then <m>n+1 \in S,</m></li>
    </ol>

    <proof>
        <p><alert>Prove:</alert> <m>\sum_{i=1}^{n} (3i-2) = \frac{n}{2}(3n-1)</m></p>
        <p><alert>Basis step:</alert> show it's true for 1</p>
        <p>Let <m>n=1</m>. Calculate <m>\sum_{i=1}^{1} (3i-2) = \frac{1}{2}(3(1)-1)</m> :</p>
        <me>3(1)-2=1</me>
        <p><alert>Inductive step:</alert> assume it's true for <m>n</m></p>
        <p><m>\sum_{i=1}^{1} (3i-2) = \frac{1}{2}(3(1)-1)</m></p>
        <me>3(1)-2=1</me>
        <p>Inductive step: (assume it's true for <m>n</m>):</p>
        <p>Let <m>n \in \mathbb{N}</m> where <m>n&gt; 1</m> and assume <m>\sum_{i=1}^{n} (3i-2) = \frac{n}{2}(3n-1)</m>.</p> 
        <p>Now we <em>show</em> it's true for <m>n+1</m>:</p>
        <p>Calculate:</p>
        <md>
            <mrow>\sum_{i=1}^{n+1} (3i-2) \amp= (\sum_{i=1}^{n} (3i-2))+(3(n+1)-2)</mrow>
            <mrow> \amp=\frac{n}{2}(3n-1)\text{ (from induction assumption) }+(3(n+1)-2)</mrow>
            <mrow> \amp=\frac{n}{2}(3n-1)+(3n+1)</mrow>
            <mrow> \amp=\frac{n}{2}(3n-1)+\frac{2}{2}(3n+1)</mrow>
            <mrow> \amp=\frac{n(3n-1)+2(3n+1)}{2}</mrow>
            <mrow> \amp=\frac{3n^2 -n+6n+2}{2}</mrow>
            <mrow> \amp=\frac{3n^2 +5n+2}{2}</mrow>
            <mrow> \amp=\frac{(n+1)(3n+2)}{2}</mrow>
            <mrow> \amp=\frac{(n+1)(3(n+1)-1}{2}</mrow>
        </md>
        <p>
            Note: Sometimes it's hard to work out the middle part...so go as far as you can in the calculation, then start at the "end"
            and work backwards until you reach where you left off.
        </p>
    </proof>

    <p>
        <alert>Principle of Complete Induction</alert>
    </p>
    <p>
        Suppose <m>S</m> is a subset of <m>\mathbb{N}</m> with the following property: <m>\forall n \in \mathbb{N}</m> if <m>\{1,2,3,...,n-1\} \subset S</m> then <m>n \in S</m>
        For this kind of proof, you start at 1, then assume <m>n-1</m>, then show <m>(n-1)+1</m>, or <m>n</m>.
    </p>
    
    <assemblage>
        <title>Fibonacci numbers</title>
        <p>
            To calculate any Fibonacci number, <m>f_n</m>, we add the two numbers that preceded it: 
        <me>
            f_n = f_{n-1} + f_{n-2}
        </me>
        </p>
        <p>
           where <m>f_1=1</m> and <m>f_2=1</m>
        </p>
    </assemblage>
    <proof>
        <p>
            <alert>Prove:</alert> <m>f_{3n}</m> is even (every third fibonacci number is even)
        </p>
        <p>
            <alert>Basis step:</alert> show it works for 1
        </p> 
        <p>
            Let <m>n=1</m>. Calculate:
            <me>
                1+1=2
            </me>
            Hence, the base case holds.
        </p>
        <p><alert>Inductive step:</alert> Let <m>n\in \mathbb{N}</m> where <m>n &gt;1</m>, and assume for
            <m>1\leq k\leq n-1</m> <m>f_{3k}</m> is even
        </p>
        <p>
            Calculate:
        </p>
        <md>
            <mrow>f_{3n}\amp=f_{3n-1}+f_{3n-2}</mrow>
            <mrow> \amp=f_{3n-2}+f_{3n-3}+f_{3n-2}</mrow>
            <mrow> \amp=2(f_{3n-2})+f_{3(n-1)}</mrow>
        </md>
        <p>
            Hence, by induction assumption, <m>f_{3(n-1)}</m> is even. Thus by definition of even, we can find an integer <m>m</m> such that <m>f_{3(n-1)}=2m</m>
        </p>
        <p>
            Calculate:
        </p>
        <md>
            <mrow>f_{3n}\amp=2f_{3n-2}+2m</mrow>
            <mrow> \amp=2(f_{3n-2+m})</mrow>
        </md>
        <p>
            Thus by definition of even, <m>f_{3n}</m> is even. Thus by proof by PCI, <m>f_{3n}</m> is even for all <m>n\in \mathbb{N}</m>
        </p>
    </proof>

    <proof>
        <p>
            <alert>Prove:</alert> <m>f_{3n+1}</m> is odd 
        </p>
        <p>
            <alert>Basis step:</alert> show it works for 1
        </p> 
        <p>
            Let <m>n=1</m>. Calculate:
            <me>
                f_{3(1)+1}=f_4
            </me>
            The fourth Fibonacci number is 3. Hence, the base case holds.
        </p>
        <p><alert>Inductive step:</alert> Let <m>n\in \mathbb{N}</m> where <m>n &gt;1</m>, and assume for
            <m>1\leq k\leq n-1</m> <m>f_{3k+1}</m> is odd
        </p>
        <p>
            Calculate:
        </p>
        <md>
            <mrow>f_{3n+1}\amp=f_{3n}+f_{3n-1}</mrow>
            <mrow> \amp=f_{3n}+f_{3n-2}+f_{3n-3}</mrow>
            <mrow> \amp=2(f_{3n})+f_{3n-2}+f_{3(n-1)}</mrow>
            <mrow> \amp=2(f_{3n})+f_{3(n-1)+1}+f_{3(n-1)}</mrow>
        </md>
        <p>
            Note: we know <m>f_{3n}</m> and <m>f_{3(n-1)}</m> are even, because we just proved it. By our induction assumption, <m>f_{3(n-1)+1}</m>
            is odd. Hence by definition of odd, we can find <m>l,m,a\in \mathbb{Z}</m> such that <m>f_{3n}=2l</m>, <m>f_{3(n-1)}=2m</m>, and
            <m>f_{3(n-1)+1}=2a+1</m>.
        </p>
        <p>
            Calculate:
        </p>
        <md>
            <mrow>f_{3n}+f_{3(n-1)+1}+f_{3(n-1)}\amp=2l+2a+1+2m</mrow>
            <mrow> \amp=2(l+a+m)+1</mrow>
        </md>
        <p>
            Thus by definition of odd, <m>f_{3n+1}</m> is odd. Thus by proof by PCI, <m>f_{3n+1}</m> is odd for all <m>n\in \mathbb{N}</m>
        </p>
    </proof>
</section>

</section>