<?xml version="1.0" encoding="UTF-8"?>

<section xml:id="sec-1-4" xmlns:xi="http://www.w3.org/2001/XInclude">
<title>Exercises</title>
<ol> 
<li>
    <p>Write truth tables for the following:</p>
    <ol>
        <li><m>(\sim P) \implies Q</m></li>
        <li><m>P \iff Q</m></li>
        <li><m>(P\vee Q)\wedge [\sim (P\wedge Q)]</m></li>
        <li><m>(P \implies Q)\vee Q</m></li>
        <li><m>(P\wedge R)\implies Q</m></li>
        <li><m>(\sim Q)\implies Q</m></li>
        <li><m>P\vee (\sim P)</m></li>
        <li><m>\sim (P\wedge Q)</m></li>
        <li><m>(\sim P)\vee (\sim Q)</m></li>
        <li><m>(\sim P)\implies (R\wedge Q)</m></li>
    </ol>
</li>
<li>
    <p>
        Show the remaining laws are from <xref ref="thm-logic-laws"/> are true, using truth tables.
    </p>
</li>
<li>
    <p>Use a truth table to show whether the following are or are not equivalent:</p>
        <ol>
            <li><m>[P\implies ((\sim Q)\wedge R)]</m>, <m>[(P\implies (\sim Q))\vee (P\implies R)]</m></li>
            <li><m>[((\sim P)\vee Q)\implies R]</m>, <m>[((\sim R)\implies P)\wedge (Q\implies R)]</m></li>
            <li><m>[(P\wedge (\sim Q)) \implies R]</m>, <m>[P\implies (Q\vee R)]</m></li>
            <li><m>[(P\implies Q)\wedge (\sim R)]</m>, <m>[(R\vee P)\implies ((\sim R)\wedge Q)]</m></li>
        </ol>
    </li>
    <li>
    <p>Turn the first statement into the second one. Show your steps and state which equivalence rule from 1.3.2 you used to get there.</p>
        <ol>
            <li><m>[P\implies ((\sim Q)\wedge R)]\equiv [(P\implies (\sim Q))\wedge (P\implies R)]</m></li>
            <li><m>[((\sim P)\vee Q)\implies R]\equiv [((\sim R)\implies P)\wedge (Q\implies R)]</m></li>
            <li><m>[(P\wedge (\sim Q))\implies R]\equiv [P\implies (Q\vee R)]</m></li>
            <li><m>[(P\implies Q)\wedge (\sim R)]\equiv [(R\vee P)\implies ((\sim R)\wedge Q)]</m></li>
        </ol>
    </li>
</ol>
</section>