<?xml version="1.0" encoding="UTF-8"?>

<section xml:id="subsec-3-5-proofs-of-or" xmlns:xi="http://www.w3.org/2001/XInclude">
<title>Proofs with Conjunctions and Disjunctions</title>
    <p>
        So far we have been proving the prototypical 
        <me>
            P\implies Q
        </me>
        as it is perhaps one of the most common propositional forms used in mathematics, and otherwise. 
        Yet, in all of our examples thus far both <m>P</m> and <m>Q</m> have been atomic propositions. In this 
        section we will be substuting the antecedent and consequent with compound propostions. 
    </p>
    <assemblage>
        <title>Assuming an Or</title>
        <p>
          For propostions <m>P</m>, <m>Q</m>, and <m>R</m>, to prove a statment in the form of 
          <me>
            (P\vee R)\implies Q
          </me>
          
        </p>
        <p>
            First we:
        </p>
        <p>
            <alert>Prove:</alert> <m>P\implies Q</m>
        </p>
        <p>
            then we:
        </p>
        <p>
            <alert>Prove:</alert> <m>R\implies Q</m>
        </p>
      </assemblage>
      <p>
        To verify that this argument is valid, we will use a truth table to show:
        <me>
            [(P\implies Q)\wedge(R\implies Q)]\implies [(P\vee R)\implies Q]
        </me>
        is a tautology.
      </p>
      <figure xml:id="assuming-or-table">
        <tabular halign="center">
            <row header="yes" bottom="minor" >
              <cell><m>P</m></cell>
              <cell><m>Q</m></cell>
              <cell><m>R</m></cell>
              <cell><m>(P\vee R)\implies Q</m></cell>
              <cell><m>[(P\implies Q)\wedge(R\implies Q)]\implies [(P\vee R)\implies Q]</m> </cell>
            </row>
            <row>
              <cell>T</cell>
              <cell>T</cell>
              <cell>T</cell>
              <cell>T</cell>
              <cell>T</cell>
            </row>
            <row>
              <cell>T</cell>
              <cell>T</cell>
              <cell>F</cell>
             <cell>T</cell>
             <cell>T</cell>
            </row>
            <row>
              <cell>T</cell>
              <cell>F</cell>
              <cell>T</cell>
              <cell>F</cell>
              <cell>T</cell>
            </row>
            <row>
              <cell>T</cell>
              <cell>F</cell>
              <cell>F</cell>
              <cell>F</cell>
              <cell>T</cell>
            </row>
            <row>
              <cell>F</cell>
              <cell>T</cell>
              <cell>T</cell>
            <cell>T</cell>
            <cell>T</cell>
            </row>
            <row>
              <cell>F</cell>
              <cell>T</cell>
              <cell>F</cell>
              <cell>T</cell>
              <cell>T</cell>
            </row>
            <row>
              <cell>F</cell>
              <cell>F</cell>
              <cell>T</cell>
            <cell>F</cell>
            <cell>T</cell>
            </row>
            <row>
              <cell>F</cell>
              <cell>F</cell>
              <cell>F</cell>
              <cell>T</cell>
              <cell>T</cell>
            </row>
          </tabular>
      </figure>
      <p>
        Now we can see an example of this in play.
      </p>
      <example>
        <p>
            <alert>Prove:</alert> for any two integers <m>x</m> and <m>y</m> if <m>x</m> is even or <m>y</m>
            is even then <m>x\cdot y</m> is even.
        </p>
       <p>
        <alert>Proof:</alert>
       </p>
       <p>
        Let <m>x</m> and <m>y</m> be integers.</p> 
        <p>
        First assume that <m>x</m> is even. By definiton of even 
        (<xref ref="defn-even"/>) we can find an integer <m>k</m> so that <m>x=2k</m>. Calculate:
        <md>
            <mrow>x\cdot y\amp=(2k)\cdot y</mrow>
            <mrow>\amp=2(ky)</mrow>
        </md>
        since <m>ky</m> is an integer by the definition of even, <m>x\cdot y</m> is even.
       </p>
       <p>
        Next, we instead assume <m>y</m> is even. By defintion of even we can find an integer <m>t</m>
        so that <m>y=2t</m>. Calculate:
        <md>
            <mrow>x\cdot y\amp=x\cdot(2t)</mrow>
            <mrow>\amp=2(xt)</mrow>
        </md>
        since <m>xt</m> is an integer by the defintion of even, <m>x\cdot y</m> is even.
       </p>
       <p>
        Now since we have shown that for <m>\forall x,y\in\Z</m> that both <m>x</m> is even implies <m>x\cdot y</m>
        is even and <m>y</m> is even implies <m>x\cdot y</m> is even,
        we have thus shown that <m>\forall x,y\in\Z</m>.
       </p>
      </example>
      <p>
        Another interesting scenerio is when we are trying to conclude a disjunction.
      </p>
      <assemblage>
        <title>Concluding an Or</title>
        <p>
          For propostions <m>P</m>, <m>Q</m>, and <m>R</m>, to prove a statment in the form of 
          <me>
            P\implies (Q\vee R)
          </me>
          
        </p>
        <p>
            We instead 
        </p>
        <p>
            <alert>Prove:</alert> <m>[P\wedge(\sim R)]\implies Q</m>
        </p>
        
      </assemblage>
      <p>
        That is argument is valid can be seen by showing that 
        <me>
            [P\implies(Q\vee R)]\equiv[[P\wedge(\sim R)]\implies Q]
        </me>
        To do that we will use the tricks of <xref ref="subsec-2-4-3-logic-algebra"/>.
      </p>
      <p>
      <md>
        <mrow>P\implies (Q\vee R)\amp \equiv [\sim P\vee( Q\vee R) \text{ (Rob's Law)}</mrow>
        <mrow>\amp \equiv [(\sim P)\vee (R\vee Q) \text{ (commutativity)}</mrow>
        <mrow>\amp \equiv [(\sim P)\vee R]\vee Q \text{ (associativity)}</mrow>
        <mrow>\amp \equiv \sim[P\wedge (\sim R)]\vee Q \text{ (De Morgan's)}</mrow>
        <mrow>\amp \equiv (P\vee R)\implies Q \text{ (Rob's Law)}</mrow>
    </md>
    </p>
</section>