<?xml version="1.0" encoding="UTF-8"?>

<section xml:id="subsec-5-1-2" xmlns:xi="http://www.w3.org/2001/XInclude">
<title>Working with Subsets</title>

<theorem xml:id="thm-5-1">
    <statement>
        <p>
            If <m>A</m> and <m>B</m> are sets with no elements, then <m>A=B</m>. In other words, the empty set is unique.
        </p>
    </statement>
</theorem>

<theorem xml:id="thm-5-2">
    <statement>
        <p>
            For any sets <m>A</m> and <m>B</m>, if <m>A \subset B</m> and <m>A \neq 0</m> then <m>B \neq 0</m>
        </p>
    </statement>
</theorem>

<theorem xml:id="thm-5-3">
    <statement>
        <p>
            For all sets <m>A</m>, <m>B</m>, and <m>C</m>:
        </p>
        <ol marker="(a)">
            <li><m>A \subset A \bigcup B</m></li>
            <li><m>A \bigcap B \subset A</m></li>
            <li><m>A \bigcap \{\} = \{\}</m></li>
            <li><m>A \bigcup \{\} = A</m></li>
            <li><m>A \bigcap A = A</m></li>
            <li><m>A \bigcup A = A</m></li>
            <li><m>A-\{\} = A</m></li>
            <li><m>\{\} - A = \{\}</m></li>
            <li><m>A \bigcup B = B \bigcup A</m> (commutativity)</li>
            <li><m>A \bigcap B = B \bigcap A</m> (commutativity)</li>
            <li><m>A \bigcup (B \bigcup C)=(A \bigcup B)\bigcup C</m> (associativity)</li>
            <li><m>A \bigcap (B \bigcap C)=(A \bigcap B)\bigcap C</m> (associativity)</li>
            <li><m>A \bigcap (B \bigcup C)=(A \bigcap B) \bigcup (A \bigcap C)</m> (distributivity)</li>
            <li><m>A \bigcup (B \bigcap C)=(A \bigcup B) \bigcap (A \bigcup C)</m> (distributivity)</li>
            <li><m>A \subset B</m> if and only if <m>A \bigcup B = B</m></li>
            <li><m>A \subset B </m> if and only if <m>A \bigcap B = A</m></li>
            <li>If <m>A \subset B</m> then <m>A \bigcup C \subset B \bigcup C</m></li>
            <li>If <m>A \subset B</m> then <m>A \bigcap C \subset B \bigcap C</m></li>
        </ol>

    </statement>
</theorem>

<theorem xml:id="thm-5-4">
    <statement>
        <ol marker="(a)">
            <li>For every set <m>A</m>, <m>\{\} \subset A</m></li>
            <li>For every set <m>A</m>, <m>A \subset A</m></li>
            <li>For all sets <m>A</m>, <m>B</m>, and <m>C</m>, if <m>A \subset B</m> and <m>B \subset C</m>, then <m>A \subset C</m></li>        
        </ol>
    </statement>
</theorem>

<p>Now we have to consider, how do we show that one set equals another, that is, <m>A=B</m>? This is another two-part proof.</p>
<ul>
    <li>Prove that <m>A \subset B</m></li>
    <li>Prove that <m>B \subset A</m></li>
    <li>Conclude that <m>A=B</m></li>
</ul>
To put it another way, <m>A=B</m> if and only if (<m>A \subset B \wedge B \subset A</m>)



</section>