<?xml version="1.0" encoding="UTF-8"?>

<section xml:id="subsec-2-4-2-important-equiv" xmlns:xi="http://www.w3.org/2001/XInclude">
    <title>Some Important Equivalences</title>
    
    
    <p>There are a number of logical equivalences that are <em>very</em> important to become familiar with. 
        We will build some of these truth tables for you, and leave the rest for exercises.
    </p>
<theorem xml:id="thm-logic-laws">
    <statement>
        <p>
        <sbsgroup widths="55% 25%"  valign="middle">
            <sidebyside>
                <p>
                    <ul>
                        <li>
                            <p>
                                <m>\sim (\sim P)\equiv P</m>
                            </p>
                        </li>
                    </ul>
                    
                </p>
                <p>
                    Double negation Law
                </p>
            </sidebyside>
            <sidebyside >
                <p>
                    <ul>
                        <li>
                            <p>
                                <m>P\wedge Q\equiv Q\wedge P</m>
                            </p>
                        </li>
                        <li>
                            <p>
                                <m>P\vee Q\equiv Q\vee P</m>
                            </p>
                        </li>
                    </ul>
                </p>
                <p>
                    Commutativity Laws
                </p>
            </sidebyside>
            <sidebyside>
                <p>
                    <ul>
                        <li><m>P\wedge (Q\vee R)\equiv (P\wedge Q)\vee (P\wedge R)</m></li>
                        <li><m>P\vee (Q\wedge R)\equiv (P\vee Q)\wedge (P\vee R)</m></li>
                    </ul>
                </p>
                <p>
                    Distributivity Laws
                </p>
            </sidebyside>
            <sidebyside>
                <p>
                    <ul>
                        <li><m>P\vee P\equiv P</m></li>
                        <li><m>P\wedge P\equiv P</m></li>
                    </ul>
                </p>
                <p>
                    Absorption Laws
                </p>
            </sidebyside>
            <sidebyside>
                <p>
                    <ul>
                        <li><m>\sim (P\vee Q)\equiv (\sim P)\wedge (\sim Q)</m></li>
                        <li><m>\sim (P\wedge Q)\equiv (\sim P)\vee (\sim Q)</m></li>
                    </ul>
                </p>
                <p>
                    DeMorgan's Law
                </p>
            </sidebyside>
            <sidebyside>
                <p>
                    <ul>
                        <li><m>(P\vee Q)\vee R\equiv P\vee (Q\vee R)</m></li>
                        <li><m>(P\wedge Q)\wedge R\equiv P\wedge (Q\wedge R)</m></li>
                    </ul>
                </p>
                <p>
                    Associativity Laws
                </p>
            </sidebyside>
            <sidebyside>
                <p>
                    <ul>
                        <li>
                            <p>
                                <m>P\implies Q\equiv (\sim P)\vee Q</m>
                            </p>
                        </li>
                    </ul>
                </p>
                <p>
                    Rob's Law
                </p>
            </sidebyside>
        </sbsgroup>
    </p>
</statement>
</theorem>

<proof>
    <p>
        We saw the double negation law in <xref ref="ex-double-negation"/>.
    </p>
    <p>
        Next we will build the truth table for Rob's Law and leave the rest as an exercise.
    </p>
    <figure>
  
        <tabular halign="center">
          <row header="yes" bottom="minor" >
            <cell><m>P</m></cell>
            <cell><m>Q</m></cell>
            <cell><m>P\implies Q</m></cell>
            <cell><m>\sim P</m></cell>
            <cell><m>(\sim P)\vee Q</m></cell>
          </row>
          <row>
            <cell>T</cell>
            <cell>T</cell>
            <cell><em>T</em></cell>
            <cell>F</cell>
            <cell><em>T</em></cell>
          </row>
          <row>
            <cell>T</cell>
            <cell>F</cell>
            <cell><em>F</em></cell>
            <cell>F</cell>
            <cell><em>F</em></cell>
          </row>
          <row>
            <cell>F</cell>
            <cell>T</cell>
            <cell><em>T</em></cell>
            <cell>T</cell>
            <cell><em>T</em></cell>
          </row>
          <row>
            <cell>F</cell>
            <cell>F</cell>
            <cell><em>T</em></cell>
            <cell>T</cell>
            <cell><em>T</em></cell>
          </row>
        </tabular>
      </figure>
</proof>


</section>