<?xml version="1.0" encoding="UTF-8"?>

<section xml:id="subsec-3-5-2-cases-examples" xmlns:xi="http://www.w3.org/2001/XInclude">
<title>Exhaustive Examples</title>
    <p>
       We now include some examples, the first one is an example 
    </p>

    <example>
        <p><alert>Prove:</alert> for any integer <m>a</m>, <m>a(a+1)</m> is even.</p>
        <p>Let <m>a</m> be an integer. <m>a</m> is either even, or odd.</p>
        <p><alert>Case 1:</alert> Assume <m>a</m> is even.</p>
        <p>Hence by definition of even, we can find an integer <m>k</m> such that <m>a=2k</m>.</p>
        <p>Calculate:</p>
        <md>
            <mrow>a(a+1)\amp=2k(2k+1)</mrow>
            <mrow>\amp=4k^2+2k</mrow>
            <mrow>2(k*k+k)</mrow>
        </md>
        <p>Thus, since <m>k^2+k</m> is an integer, by definition of even, <m>a(a+1)</m> is even. Thus by direct proof, 
            if <m>a</m> is even then <m>a(a+1)</m> is even.</p>
        <p><alert>Case 2:</alert> Assume <m>a</m> is odd. Thus by definitino of odd, we can find an integer <m>m</m> such that <m>a=2m+1</m></p>
        <p>Calculate</p>
        <md>
            <mrow>a(a+1)\amp=(2m+1)(2m+1+1)</mrow>
            <mrow>\amp=(2m+1)(2(m+1))</mrow>
            <mrow>2[(2m+1)(2m+1)</mrow>
        </md>
        <p>Thus since <m>(2m+1)(2m+1)</m> is an integer, according to the definition of even, <m>a(a+1)</m> is even. Thus by direct proof 
        if <m>a</m> is odd then <m>a(a+1)</m> is even.</p>
        <p>Thus since case 1 and case 2 hold, by proof by cases, and by direct proof, <m>a(a+1)</m> is even. <m>\square</m></p>
    </example>

    <example>
        <p><alert>Prove:</alert> for any integer <m>n</m>, if <m>n</m> is odd, then there exists an integer <m>j</m> so 
            that <m>n=4j-1</m> or <m>n=4j+1</m></p>
        <p>Let <m>n</m> be an integer. Assume <m>n</m> is odd. By definition of odd we can find an integer <m>m</m> such that <m>n=2m+1</m></p>>
        <p><alert>Case 1:</alert> Assume <m>m</m> is even. By definition of even we can find an integer <m>j</m> such that <m>m=2j</m>.</p>
        Calculate:
        <md>
            <mrow>n\amp=2m+1</mrow>
            <mrow>\amp=2(2j)+1</mrow>
            <mrow>\amp=4j+1</mrow>
        </md>
        <p>Hence case 1 holds by direct proof.</p>
        <p><alert>Case 2:</alert> Assume <m>m</m> is odd. Thus by definition of odd we can find an integer <m>k</m> so taht <m>m=2k+1</m></p>
        <p>Calculate:</p>
        <md>
            <mrow>n\amp=2n+1</mrow>
            <mrow>\amp=2(2k+1)</mrow>
            <mrow>\amp=4k+3</mrow>
            <mrow>\amp=4k+4-2</mrow>
            <mrow>\amp=4(k+1)-1</mrow>
        </md>
        <p>Hence case 2 holds by direct proof.</p>
        <p>Thus, since case 1 and case 2 hold, by proof by cases, if <m>n</m> is odd, then we can find an 
            integer<m>j</m> so that <m>n=4j-1</m> or <m>n=4j+1</m></p>
    </example>

</section>