<md>
    <mrow>x+y\amp=(2t+1)+(2s+1)</mrow>
    <mrow>\amp=2s+2t+1+1</mrow>
    <mrow>\amp=2s+2t+2</mrow>
    <mrow>\amp=2(s+t+1)</mrow>
</md>

arguments:

    <tabular halign="center">
    <row>
      <cell><m>A</m></cell>
    </row>
    <row  bottom="minor">
      <cell><m>B</m></cell>
    </row>
    <row>
      <cell><m>\therefore C</m></cell>
    </row>
    </tabular>

    truth table:

    <figure>
        <tabular halign="center">
          <row header="yes" bottom="minor" >
            <cell><m>P</m></cell>
            <cell><m>Q</m></cell>
            <cell><m>P\implies Q</m></cell>
          </row>
          <row>
            <cell>T</cell>
            <cell>T</cell>
            <cell>T</cell>
          </row>
          <row>
            <cell>T</cell>
            <cell>F</cell>
            <cell>F</cell>
          </row>
          <row>
            <cell>F</cell>
            <cell>T</cell>
            <cell>T</cell>
          </row>
          <row>
            <cell>F</cell>
            <cell>F</cell>
            <cell>T</cell>
          </row>
        </tabular>
      
    </figure>